TM/Compound/Peek.v
@@ -11,23 +11,23 @@ Section Peek.
   Variable f : sig -> F.
 
   Definition Peek : { M : mTM sig 1 & states M -> F + move } :=
-    MATCH (Read_char _)
+    MATCH (Read_char)
           (fun r1 =>
              match r1 with
-             | Some r1' => mono_Nop sig (inl (f r1'))
+             | Some r1' => mono_Nop (inl (f r1'))
              | None =>
-               Move sig L tt ;;
-                    MATCH (Read_char _)
+               Move L tt ;;
+                    MATCH (Read_char)
                     (fun r2 =>
                        match r2 with
-                       | Some r2' => Move sig R (inr R)
+                       | Some r2' => Move R (inr R)
                        | None =>
-                         Move sig R tt ;;
-                              MATCH (Read_char _)
+                         Move R tt ;;
+                              MATCH (Read_char)
                               (fun r3 =>
                                  match r3 with
-                                 | Some r3' => Move sig L (inr L)
-                                 | None => mono_Nop sig (inr N)
+                                 | Some r3' => Move L (inr L)
+                                 | None => mono_Nop (inr N)
                                  end)
                        end)
              end).
